proof: use the solve-simp tactic

cogent/isa/CogentHelper.thy
@@ -121,20 +121,20 @@ lemma ttsplit_weak_lemma:
     \<Longrightarrow> type_ctx_wellformed K (snd \<Gamma>1)
     \<Longrightarrow> type_ctx_wellformed K (snd \<Gamma>2)
     \<Longrightarrow> ttsplit K \<Gamma> sps xs \<Gamma>1 ys \<Gamma>2"
-  apply (clarsimp_solve simp: ttsplit_def ttsplit_weak_def type_ctx_wellformed_def)
-  apply (clarsimp_solve simp_solve add: ttsplit_inner_def)
-  apply (clarsimp_solve simp: ttsplit_inner_def in_set_conv_nth all_conj_distrib)
-  apply (clarsimp_solve simp: image_def Product_Type.split_def set_zip)
+  apply (clarsimp simp: ttsplit_def ttsplit_weak_def type_ctx_wellformed_def)
+  apply (clarsimp simp add: ttsplit_inner_def)
+  apply (clarsimp simp: ttsplit_inner_def in_set_conv_nth all_conj_distrib)
+  apply (clarsimp simp: image_def Product_Type.split_def set_zip)
   apply (drule_tac x=y in spec)+
   apply clarsimp
   apply (drule_tac x=i in spec)+
-  apply (clarsimp_solve split: if_splits)
+  apply (clarsimp split: if_splits)
   done
 
 lemma ttsplit_weakI:
   "ttsplit_inner K sps False \<Gamma>b \<Gamma>1 \<Gamma>2 \<Longrightarrow> xs' = xs @ \<Gamma>1 \<Longrightarrow> ys' = ys @ \<Gamma>2
     \<Longrightarrow> ttsplit_weak K (TyTrSplit sps xs T1 ys T2, \<Gamma>b) sps xs (T1, xs') ys (T2, ys')"
-  by (simp_solve add: ttsplit_weak_def)
+  by (simp add: ttsplit_weak_def)
 *)
 
 lemmas ttyping_type_ctx_wellformed = ttyping_type_wellformed[folded type_ctx_wellformed_def]
@@ -337,13 +337,13 @@ fun ttsplit_inner (@{term "Some TSK_S"} :: tsks) (SOME p :: Gamma) = let
   in [RTac @{thm ttsplit_innerI(4)}, ForceTac @{thms kinding_defs}] @ rest end
   | ttsplit_inner (@{term "Some TSK_L"} :: tsks) (SOME p :: Gamma) = let
     val rest = ttsplit_inner tsks Gamma
-  in [RTac @{thm ttsplit_innerI(3)}, simp] @ rest end
+  in [RTac @{thm ttsplit_innerI(3)}, simp_solve] @ rest end
   | ttsplit_inner (@{term "Some TSK_R :: type_split_op option"} :: tsks) (SOME p :: Gamma) = let
     val rest = ttsplit_inner tsks Gamma
-  in [RTac @{thm ttsplit_innerI(2)}, simp] @ rest end
+  in [RTac @{thm ttsplit_innerI(2)}, simp_solve] @ rest end
   | ttsplit_inner (@{term "Some TSK_NS :: type_split_op option"} :: tsks) (SOME p :: Gamma) = let
     val rest = ttsplit_inner tsks Gamma
-  in [RTac @{thm ttsplit_innerI(5)}, simp] @ rest end
+  in [RTac @{thm ttsplit_innerI(5)}, simp_solve] @ rest end
   | ttsplit_inner (@{term "None :: type_split_op option"} :: tsks) (NONE :: Gamma) = let
     val rest = ttsplit_inner tsks Gamma
   in [RTac @{thm ttsplit_innerI(1)}] @ rest end
@@ -352,12 +352,12 @@ fun ttsplit_inner (@{term "Some TSK_S"} :: tsks) (SOME p :: Gamma) = let
 
 fun ttsplit (Const (@{const_name TyTrSplit}, _) $ sps $ _ $ _ $ _ $ _, Gamma) = let
     val inner = ttsplit_inner (HOLogic.dest_list sps) Gamma
-  in [RTac @{thm ttsplitI}] @ inner @ [simp, simp, simp] end
+  in [RTac @{thm ttsplitI}] @ inner @ [simp_solve, simp_solve, simp_solve] end
   | ttsplit (t, _) = raise TERM ("ttsplit", [t])
 
 fun ttsplit_bang (Const (@{const_name TyTrSplit}, _) $ sps $ _ $ _ $ _ $ _, Gamma) = let
     val inner = ttsplit_inner (HOLogic.dest_list sps) Gamma
-  in [RTac @{thm ttsplit_bangI}, simp, simp, SimpTac (@{thms set_eq_subset}, [])] @ inner end
+  in [RTac @{thm ttsplit_bangI}, simp_solve, simp_solve, SimpTac (@{thms set_eq_subset}, [])] @ inner end
   | ttsplit_bang (t, _) = raise TERM ("ttsplit", [t])
 
 fun dest_nat (@{term Suc} $ n) = dest_nat n + 1
@@ -375,15 +375,15 @@ fun the_G _ (SOME p) = p
   | the_G G NONE = raise THM ("the_G", 1, (map (fn NONE => @{thm TrueI} | SOME t => t) G))
 
 fun typing_all_vars _ _ [] = let
-  in [RTac @{thm typing_all_empty''}, simp] end
+  in [RTac @{thm typing_all_empty''}, simp_solve] end
   | typing_all_vars ctxt G (ix :: ixs) = let
     fun null (NONE : thm option) = true
       | null _ = false
     fun step (i, p) = RTac @{thm split_cons} :: (if member (op =) ixs i
       then (if i = ix then [RTac @{thm split_comp.share}, ForceTac @{thms kinding_defs}]
-          else [RTac @{thm split_comp.right}, simp])
+          else [RTac @{thm split_comp.right}, simp_solve])
       else (if null p then [RTac @{thm split_comp.none}]
-          else [RTac @{thm split_comp.left}, simp]))
+          else [RTac @{thm split_comp.left}, simp_solve]))
     val enumG = (0 upto (length G - 1) ~~ G)
     val steps = maps step enumG
     val thms = map_filter I G
@@ -392,7 +392,7 @@ fun typing_all_vars _ _ [] = let
     val rest = typing_all_vars ctxt G' ixs
   in [RTac @{thm typing_all_cons}] @ steps @ [RTac @{thm split_empty},
     RTac @{thm typing_var_weak[unfolded singleton_def Cogent.empty_def]},
-      RTac (the_G G (nth G ix)), simp, WeakeningTac thms, simp] @ rest end
+      RTac (the_G G (nth G ix)), simp, WeakeningTac thms, simp_solve] @ rest end
 
 fun typing (Const (@{const_name Var}, _) $ i) G _ hints = let
     val i = dest_nat i
@@ -402,20 +402,20 @@ fun typing (Const (@{const_name Var}, _) $ i) G _ hints = let
                [] => ()
              | _ => raise HINTS ("too many tacs", hints))
   in ([RTac @{thm typing_var_weak[unfolded singleton_def Cogent.empty_def]},
-                RTac thm, simp, WeakeningTac thms, simp]) end
+                RTac thm, simp, WeakeningTac thms, simp_solve]) end
   | typing (Const (@{const_name Struct}, _) $ _ $ xs) G ctxt hints
   = (case dest_all_vars xs of SOME ixs => let
       val _ = (case typing_hint hints of
                  [] => ()
                | _ => raise HINTS ("too many tacs", hints))
-  in ([RTac @{thm typing_struct'}] @ typing_all_vars ctxt G ixs @ [simp, simp, simp, simp]) end
+  in ([RTac @{thm typing_struct'}] @ typing_all_vars ctxt G ixs @ [simp_solve, simp_solve, simp_solve, simp_solve]) end
     | NONE => typing_hint hints)
   | typing (Const (@{const_name Prim}, _) $ _ $ xs) G ctxt hints
   = (case dest_all_vars xs of SOME ixs => let
     val _ = (case typing_hint hints of
                [] => ()
              | _ => raise HINTS ("too many tacs", hints))
-  in ([RTac @{thm typing_prim'}, simp, simp] @ typing_all_vars ctxt G ixs) end
+  in ([RTac @{thm typing_prim'}, simp_solve, simp_solve] @ typing_all_vars ctxt G ixs) end
     | NONE => typing_hint hints)
   | typing (Const (@{const_name Promote}, _) $ _ $ e) G ctxt hints =
     ([RTac @{thm typing_promote}] @ typing e G ctxt hints @ [ForceTac @{thms subtyping_simps kinding_defs}])
@@ -456,7 +456,7 @@ fun ttyping (Const (@{const_name Split}, _) $ x $ y) tt k ctxt hint_tree = let
     val x_tac = ttyping x ltt k ctxt typxhint
     val y_tac = ttyping y rtt k ctxt typyhint
     val k_tac = kinding kindhint
-  in ([RTac @{thm ttyping_letb}] @ tsb_tac @ x_tac @ y_tac @ k_tac @ [simp]) end
+  in ([RTac @{thm ttyping_letb}] @ tsb_tac @ x_tac @ y_tac @ k_tac @ [simp_solve]) end
   | ttyping (Const (@{const_name Cogent.If}, _) $ c $ x $ y) tt k ctxt hint_tree = let
     val (typxhint, splithints, typahint, typbhint) = (case hint_tree of
         Branch [typxhint, Branch splithints, typahint, typbhint] =>
@@ -473,7 +473,7 @@ fun ttyping (Const (@{const_name Split}, _) $ x $ y) tt k ctxt hint_tree = let
     val x_tac = ttyping x x_tt k ctxt typahint
     val y_tac = ttyping y y_tt k ctxt typbhint
   in ([RTac @{thm ttyping_if}] @ split_tac
-    @ [simp, RTac @{thm ttsplit_trivI}, simp, simp] @ c_tac @ x_tac @ y_tac) end
+    @ [simp, RTac @{thm ttsplit_trivI}, simp_solve, simp_solve] @ c_tac @ x_tac @ y_tac) end
   | ttyping (Const (@{const_name Case}, _) $ x $ _ $ m $ nm) tt k ctxt hint_tree = let
     val (typxhint, splithints, typahint, typbhint) = (case hint_tree of
         Branch [typxhint, Branch splithints, typahint, typbhint] =>
@@ -487,8 +487,8 @@ fun ttyping (Const (@{const_name Split}, _) $ x $ y) tt k ctxt hint_tree = let
     val split_tac = ttsplit tt
     val m_tac = ttyping m m_tt k ctxt typahint
     val nm_tac = ttyping nm nm_tt k ctxt typbhint
-  in ([RTac @{thm ttyping_case'}] @ split_tac @ x_tac @ [simp]
-    @ [simp, RTac @{thm ttsplit_trivI}, simp, simp] @ m_tac @ nm_tac) end
+  in ([RTac @{thm ttyping_case'}] @ split_tac @ x_tac @ [simp_solve]
+    @ [simp, RTac @{thm ttsplit_trivI}, simp_solve, simp_solve] @ m_tac @ nm_tac) end
   | ttyping (Const (@{const_name Take}, _) $ x $ _ $ y) tt k ctxt hint_tree = let
     val (splithints, typehint, kindhint, type'hint) = (case hint_tree of
         Branch [Branch splithints, typehint, kindhint, type'hint] =>
@@ -502,7 +502,7 @@ fun ttyping (Const (@{const_name Split}, _) $ x $ y) tt k ctxt hint_tree = let
     val k_tac = kinding kindhint
     val y_tac = ttyping y rtt k ctxt type'hint
   in ([RTac @{thm ttyping_take'}] @ split_tac @ x_tac
-    @ [simp, simp, simp] @ k_tac @ [simp] @ y_tac) end
+    @ [simp_solve, simp_solve, simp_solve] @ k_tac @ [simp_solve] @ y_tac) end
   | ttyping x (@{term TyTrLeaf}, G) _ ctxt hint_tree = let
     val ty_tac = typing x G ctxt hint_tree
   in ([RTac @{thm ttyping_default}, SimpTac (@{thms composite_anormal_expr_def}, [])] @ ty_tac) end
